\chapter{Series}

\section{Series}

\begin{definition}[Series]
  Series is the sum of the terms of a sequence.
  \[
    a_{1} + a_{2} + a_{3} + \dots + a_{n}
  \]
\end{definition}

\begin{definition}[Infinite Series]
  An infinite series is the sum of the terms of an infinite sequence.
  \[
    a_{1} + a_{2} + a_{3} + \dots + a_{n} + \dots
  \]
\end{definition}

In this chapter we will try testing the convergence of the series.

\begin{definition}
  Given a series \(\sum_{n = 1}^{\infty} a_{n} = a_{1} + a_{2} + \dots\), let \(s_{n}\) denote its nth partial sum:
  \[
    s_{n} = \sum_{i = 1}^{n} = a_{1} + a_{2} + \dots + a_{n}
  \]
\end{definition}

\begin{lemma}
  \[
    \sum_{n = 1}^{\infty} a_{n} = \lim_{n \to \infty} \sum_{i=1}^{n} a_{i}
  \]
\end{lemma}

Sometimes $s_{n}$ is expressing in telescoping sum form. For example

\begin{equation}
  \nonumber
  \begin{aligned}
    \sum_{n=1}^{\infty} \ln{\frac{n}{n + 1}} &= \sum_{n=1}^{\infty} \ln{n} - \ln{(n + 1)} \\
    &= \lim_{n \to \infty} (\ln{1} - \ln{2}) + (\ln{2} - \ln{3}) + (\ln{3} - \ln{4}) + \dots + (\ln{n} - \ln{(n + 1)}) \\
    &= \lim_{n \to \infty} \ln{1} - \ln{(n + 1)} \\
    &= \lim_{n \to \infty} \ln{\frac{1}{n + 1}} \\
    &= \ln{0} \\
    &= -\infty
  \end{aligned}
\end{equation}

Such that, $\sum_{n=1}^{\infty} \ln{\frac{n}{n + 1}}$ is divergent.

\begin{equation}
  \nonumber
  \begin{aligned}
    \sum_{n=1}^{\infty} (e^{1/n} - e^{1/(n + 1)}) &= \sum_{n=1}^{\infty}(\sqrt[n]{e} - \sqrt[n + 1]{e}) \\
    &= \lim_{n \to \infty} (e - \sqrt{e}) + (\sqrt{e} - \sqrt[3]{e}) + (\sqrt[3]{e} - \sqrt[4]{e}) + \dots + (\sqrt[n]{e} - \sqrt[n + 1]{e})\\
    &= \lim_{n \to \infty} e - \sqrt[n + 1]{e} \\
    &= e - e^{0} \\
    &= e - 1
  \end{aligned}
\end{equation}

Such that, $\sum_{n=1}^{\infty} (e^{1/n} - e^{1/(n + 1)})$ converges to $e - 1$.

\section{Geometric Series}

\begin{definition}
  \[
    a + ar + ar^{2} + \dots + ar^{n-1} + \dots = \sum_{n = 1}^{\infty} ar^{n-1} \; \text{where} \; a \neq 0
  \]
  is defined as a geometric series which \(a\) is the first term and \(r\) is the common ratio.
  \[
    r = \frac{a_{n+1}}{a_{n}}, \; n \geq 1
  \]
\end{definition}

\begin{lemma}
  If \(|r| \neq 1\), we have
  \begin{equation}
    \nonumber
    \begin{aligned}
      s_{n} &= a + ar + ar^{2} + \dots + ar^{n - 1} \\
      r \cdot s_{n} &= a_r + ar^{2} + ar^{3} + \dots + ar^{n} \\
      s_{n} - r \cdot s_{n} &= a - ar^{n} \\
      s_{n} &= \frac{a(1 - r^{n})}{1 - r}
    \end{aligned}
  \end{equation}
\end{lemma}

\begin{lemma}
  The geometric series
  \[
    \sum_{n = 1}^{\infty} ar^{n-1} = a + ar + ar^{2} + \dots + ar^{n-1} + \dots
  \]
  is convergent if \(|r| < 1\) and its sum is
  \[
    \sum_{n = 1}^{\infty} ar^{n-1} = \frac{a}{1 - r}  
  \]
  If \(|r| \geq 1\), the series is divergent.
\end{lemma}

\begin{proof}
  If \(|r| < 1\), we have
  \begin{equation}
    \nonumber
    \begin{aligned}
      \lim_{n \to \infty} s_{n} &= \lim_{n \to \infty} \frac{a(1 - r^{n})}{1 - r} \\
      &= \frac{a}{1 - r} - \frac{a}{1 - r} \cdot \lim_{n \to \infty} r^{n} \\
      &= \frac{a}{1 - r} - \frac{a}{1 - r} \cdot 0 \\
      &= \frac{a}{1 - r}
    \end{aligned}
  \end{equation}
  If \(|r| \geq 1\), we have \(\lim_{n \to \infty} r^{n} = \infty\), such that the series is divergent.
\end{proof}